src/program_proof/simple/example.v
@@ -1,7 +1,7 @@
 From RecordUpdate Require Import RecordSet.
 Import RecordSetNotations.
 
-From Perennial.algebra Require Import deletable_heap liftable auth_map.
+From Perennial.algebra Require Import liftable auth_map.
 From Perennial.Helpers Require Import Transitions.
 From Perennial.program_proof Require Import proof_prelude.
 
@@ -20,7 +20,6 @@ From Perennial.goose_lang Require wpr_lifting.
 
 Section heap.
 Context `{!heapG Σ}.
-Context `{!gen_heapPreG u64 bool Σ}.
 Context `{!simpleG Σ}.
 Implicit Types (stk:stuckness) (E: coPset).
 
@@ -123,7 +122,6 @@ Import wpr_lifting.
 
 Section recov.
   Context `{!heapG Σ}.
-  Context `{!gen_heapPreG u64 bool Σ}.
   Context `{!simpleG Σ}.
 
   (* Just a simple example of using idempotence *)
